theories/models/utp_cml/utp_cml_functions.thy
@@ -48,10 +48,10 @@ definition "vexpr_hd      = Op1DR {x. x \<noteq> []} hd"
 definition "vexpr_tl      = Op1DR {x. x \<noteq> []} tl"
 definition "vexpr_seqapp  = Op2DR {(xs, i::real). i \<in> Nats \<and> nat (floor i) < length xs} (\<lambda> xs i. nth xs (nat (floor i)))"
 
-definition vexpr_seqcomp :: "('a option \<Rightarrow> 'b::{vbasic,linorder} cmle * bool cmle) \<Rightarrow> 'a fset cmle \<Rightarrow> 'b list cmle" where
+definition vexpr_seqcomp :: "('a \<Rightarrow> 'b::{vbasic,linorder} cmle * bool cmle) \<Rightarrow> 'a fset cmle \<Rightarrow> 'b list cmle" where
 "vexpr_seqcomp FP eA = do { A <- eA
-                          ; PA <- cmle_fset_iter A (\<lambda> x. do { c <- snd(FP(Some(x))); if c then LitD \<lbrace>x\<rbrace> else LitD \<lbrace>\<rbrace> })
-                          ; LA <- cmle_fset_iter (\<Union>\<^sub>f PA) (fst \<circ> FP \<circ> Some)
+                          ; PA <- cmle_fset_iter A (\<lambda> x. do { c <- snd(FP(x)); if c then LitD \<lbrace>x\<rbrace> else LitD \<lbrace>\<rbrace> })
+                          ; LA <- cmle_fset_iter (\<Union>\<^sub>f PA) (fst \<circ> FP)
                           ; LitD (flist LA) }"
 
 definition vexpr_subseq :: "'a list cmle \<Rightarrow> real cmle \<Rightarrow> real cmle \<Rightarrow> 'a list cmle" where
@@ -114,19 +114,19 @@ lift_definition fatLeastAtMost :: "int \<Rightarrow> int \<Rightarrow> int fset"
 definition vexpr_set_range :: "real cmle \<Rightarrow> real cmle \<Rightarrow> real fset cmle" where
 "vexpr_set_range = Op2D' (\<lambda> m n. real `\<^sub>f fatLeastAtMost (floor m) (floor n))"
 
-definition vexpr_setcomp :: "('a option \<Rightarrow> 'b::{vbasic,linorder} cmle * bool cmle) \<Rightarrow> 'a fset cmle \<Rightarrow> 'b fset cmle" where
+definition vexpr_setcomp :: "('a \<Rightarrow> 'b::{vbasic,linorder} cmle * bool cmle) \<Rightarrow> 'a fset cmle \<Rightarrow> 'b fset cmle" where
 "vexpr_setcomp FP eA = do { A <- eA
-                          ; PA <- cmle_fset_iter A (\<lambda> x. do { c <- snd(FP(Some(x))); if c then LitD \<lbrace>x\<rbrace> else LitD \<lbrace>\<rbrace> })
-                          ; LA <- cmle_fset_iter (\<Union>\<^sub>f PA) (fst \<circ> FP \<circ> Some)
+                          ; PA <- cmle_fset_iter A (\<lambda> x. do { c <- snd(FP(x)); if c then LitD \<lbrace>x\<rbrace> else LitD \<lbrace>\<rbrace> })
+                          ; LA <- cmle_fset_iter (\<Union>\<^sub>f PA) (fst \<circ> FP)
                           ; LitD LA }"
 
 declare vexpr_setcomp_def [evalp]
 
-definition ForallSetD :: "'a fset cmle \<Rightarrow> ('a option \<Rightarrow> bool cmle) \<Rightarrow> bool cmle" where
-"ForallSetD xs f = MkPExpr (\<lambda> b. (Some (\<forall> x \<in> \<langle>the (\<lbrakk>xs\<rbrakk>\<^sub>* b)\<rangle>\<^sub>f. \<lbrakk>f (Some x)\<rbrakk>\<^sub>* b = Some True)))"
+definition ForallSetD :: "'a fset cmle \<Rightarrow> ('a \<Rightarrow> bool cmle) \<Rightarrow> bool cmle" where
+"ForallSetD xs f = MkPExpr (\<lambda> b. (Some (\<forall> x \<in> \<langle>the (\<lbrakk>xs\<rbrakk>\<^sub>* b)\<rangle>\<^sub>f. \<lbrakk>f(x)\<rbrakk>\<^sub>* b = Some True)))"
 
-definition ExistsSetD :: "'a fset cmle \<Rightarrow> ('a option \<Rightarrow> bool cmle) \<Rightarrow> bool cmle" where
-"ExistsSetD xs f = MkPExpr (\<lambda> b. (Some (\<exists> x \<in> \<langle>the (\<lbrakk>xs\<rbrakk>\<^sub>* b)\<rangle>\<^sub>f. \<lbrakk>f (Some x)\<rbrakk>\<^sub>* b = Some True)))"
+definition ExistsSetD :: "'a fset cmle \<Rightarrow> ('a \<Rightarrow> bool cmle) \<Rightarrow> bool cmle" where
+"ExistsSetD xs f = MkPExpr (\<lambda> b. (Some (\<exists> x \<in> \<langle>the (\<lbrakk>xs\<rbrakk>\<^sub>* b)\<rangle>\<^sub>f. \<lbrakk>f(x)\<rbrakk>\<^sub>* b = Some True)))"
 
 definition FCollect :: "('a \<Rightarrow> bool option) \<Rightarrow> 'a fset option" where
 "FCollect p = (if (finite (Collect (the \<circ> p)) \<and> None \<notin> range p) then Some (Abs_fset (Collect (the \<circ> p))) else None)"
@@ -158,8 +158,8 @@ definition vcollect :: "('a \<Rightarrow> bool cmle) \<Rightarrow> 'a fset cmle"
 definition vcollect_ext :: "('a \<Rightarrow> 'b cmle) \<Rightarrow> ('a \<Rightarrow> bool cmle) \<Rightarrow> 'b fset cmle" where
 "vcollect_ext f P = MkPExpr (\<lambda> b. FCollect_ext (\<lambda> x. \<lbrakk>f(x)\<rbrakk>\<^sub>*b) (\<lambda> x. \<lbrakk>P(x)\<rbrakk>\<^sub>*b))"
 
-abbreviation vcollect_ext_ty :: "('a option \<Rightarrow> 'b cmle) \<Rightarrow> 'a set \<Rightarrow> ('a option \<Rightarrow> bool cmle) \<Rightarrow> 'b fset cmle" where
-"vcollect_ext_ty f A P \<equiv> vcollect_ext (f \<circ> Some) (\<lambda> x. AndD (P (Some x)) (LitD (x \<in> A)))"
+abbreviation vcollect_ext_ty :: "('a \<Rightarrow> 'b cmle) \<Rightarrow> 'a set \<Rightarrow> ('a \<Rightarrow> bool cmle) \<Rightarrow> 'b fset cmle" where
+"vcollect_ext_ty f A P \<equiv> vcollect_ext f (\<lambda> x. AndD (P(x)) (LitD (x \<in> A)))"
 
 syntax
   "_vexpr_quotev"  :: "string \<Rightarrow> n_pexpr" ("<_>")
@@ -488,7 +488,7 @@ term "|{ &x + 1 | x : @nat @ &x > 1}|"
 lemma "|{ &x | x : @real @ &x in @set &xs}| = |&xs|"
   apply (simp add:vcollect_ext_def evalp)
   apply (case_tac xs)
-  apply (auto simp add:FCollect_def)
+  apply (auto simp add:FCollect_def fsets_def)
 done
 
 lemma FUnion_finsert [simp]: 
